theories/opsem.v
@@ -3,7 +3,7 @@
 (* (C) J. Pichon, M. Bodin - see LICENSE.txt *)
 
 From Coq Require Import ZArith.BinInt NArith.BinNat.
-From mathcomp Require Import ssreflect ssrfun ssrnat ssrbool eqtype seq.
+From mathcomp Require Import ssreflect ssrfun ssrbool eqtype ssrnat seq.
 Require Export operations host.
 
 Set Implicit Arguments.
@@ -24,343 +24,488 @@ Let host_state := host_state host_instance.
 Inductive reduce_simple : seq administrative_instruction -> seq administrative_instruction -> Prop :=
 
 (** unop **)
-  | rs_unop : forall v op t,
+| rs_unop : forall v op t,
     reduce_simple [::$VA v; AI_basic (BI_unop t op)] [::$VA (@app_unop op v)]
-                   
+                  
 (** binop **)
-  | rs_binop_success : forall v1 v2 v op t,
+| rs_binop_success : forall v1 v2 v op t,
     app_binop op v1 v2 = Some v ->
     reduce_simple [::$VA v1; $VA v2; AI_basic (BI_binop t op)] [::$VA v]
-  | rs_binop_failure : forall v1 v2 op t,
+| rs_binop_failure : forall v1 v2 op t,
     app_binop op v1 v2 = None ->
     reduce_simple [::$VA v1; $VA v2; AI_basic (BI_binop t op)] [::AI_trap]
                   
-  (** testops **)
-  | rs_testop_i32 :
-    forall c testop,
+(** testops **)
+| rs_testop_i32 :
+  forall c testop,
     reduce_simple [::$VA (VAL_int32 c); AI_basic (BI_testop T_i32 testop)] [::$VA (VAL_int32 (wasm_bool (@app_testop_i i32t testop c)))]
-  | rs_testop_i64 :
-    forall c testop,
+| rs_testop_i64 :
+  forall c testop,
     reduce_simple [::$VA (VAL_int64 c); AI_basic (BI_testop T_i64 testop)] [::$VA (VAL_int32 (wasm_bool (@app_testop_i i64t testop c)))]
 
-  (** relops **)
-  | rs_relop: forall v1 v2 t op,
+(** relops **)
+| rs_relop: forall v1 v2 t op,
     reduce_simple [::$VA v1; $VA v2; AI_basic (BI_relop t op)] [::$VA (VAL_int32 (wasm_bool (app_relop op v1 v2)))]
-                    
-  (** convert and reinterpret **)
-  | rs_convert_success :
-    forall t1 t2 v v' sx,
+                  
+(** convert and reinterpret **)
+| rs_convert_success :
+  forall t1 t2 v v' sx,
     types_agree (T_num t1) (VAL_num v) ->
     cvt t2 sx v = Some v' ->
     reduce_simple [::$VA v; AI_basic (BI_cvtop t2 CVO_convert t1 sx)] [::$VA v']
-  | rs_convert_failure :
-    forall t1 t2 v sx,
+| rs_convert_failure :
+  forall t1 t2 v sx,
     types_agree (T_num t1) (VAL_num v) ->
     cvt t2 sx v = None ->
     reduce_simple [::$VA v; AI_basic (BI_cvtop t2 CVO_convert t1 sx)] [::AI_trap]
-  | rs_reinterpret :
-    forall t1 t2 v,
+| rs_reinterpret :
+  forall t1 t2 v,
     types_agree (T_num t1) (VAL_num v) ->
     reduce_simple [::$VA v; AI_basic (BI_cvtop t2 CVO_reinterpret t1 None)] [::$VA (wasm_deserialise (bits v) t2)]
 
-  (** control-flow operations **)
-  | rs_unreachable :
-    reduce_simple [::AI_basic BI_unreachable] [::AI_trap]
-  | rs_nop :
-    reduce_simple [::AI_basic BI_nop] [::]
-  | rs_drop :
-    forall v,
+(** control-flow operations **)
+| rs_unreachable :
+  reduce_simple [::AI_basic BI_unreachable] [::AI_trap]
+| rs_nop :
+  reduce_simple [::AI_basic BI_nop] [::]
+| rs_drop :
+  forall v,
     reduce_simple [::$VA v; AI_basic BI_drop] [::]
-  | rs_select_false :
-    forall n v1 v2 ot,
+| rs_select_false :
+  forall n v1 v2 ot,
     n = Wasm_int.int_zero i32m ->
     reduce_simple [::$VA v1; $VA v2; $VA (VAL_int32 n); AI_basic (BI_select ot)] [::$VA v2]
-  | rs_select_true :
-    forall n v1 v2 ot,
+| rs_select_true :
+  forall n v1 v2 ot,
     n <> Wasm_int.int_zero i32m ->
     reduce_simple [::$VA v1; $VA v2; $VA (VAL_int32 n); AI_basic (BI_select ot)] [::$VA v1]
-  | rs_label_const :
-      forall n es vs,
-        const_list vs ->
-        reduce_simple [::AI_label n es vs] vs
-  | rs_label_trap :
-      forall n es,
-        reduce_simple [::AI_label n es [::AI_trap]] [::AI_trap]
-  | rs_br :
-      forall n vs es (i: labelidx) LI (lh: lholed i),
-        const_list vs ->
-        length vs = n ->
-        lfilled lh (vs ++ [::AI_basic (BI_br i)]) LI ->
-        reduce_simple [::AI_label n es LI] (vs ++ es)
-  | rs_br_if_false :
-      forall n i,
-        n = Wasm_int.int_zero i32m ->
-        reduce_simple [::$VA (VAL_int32 n); AI_basic (BI_br_if i)] [::]
-  | rs_br_if_true :
-      forall n i,
-        n <> Wasm_int.int_zero i32m ->
-        reduce_simple [::$VA (VAL_int32 n); AI_basic (BI_br_if i)] [::AI_basic (BI_br i)]
-  | rs_br_table :
-      forall iss c i j,
-        length iss > Wasm_int.nat_of_uint i32m c ->
-        List.nth_error iss (Wasm_int.nat_of_uint i32m c) = Some j ->
-        reduce_simple [::$VA (VAL_int32 c); AI_basic (BI_br_table iss i)] [::AI_basic (BI_br j)]
-  | rs_br_table_length :
-      forall iss c i,
-        length iss <= (Wasm_int.nat_of_uint i32m c) ->
-        reduce_simple [::$VA (VAL_int32 c); AI_basic (BI_br_table iss i)] [::AI_basic (BI_br i)]
-  | rs_local_const :
-      forall es n f,
-        const_list es ->
-        length es = n ->
-        reduce_simple [::AI_local n f es] es
-  | rs_local_trap :
-      forall n f,
-        reduce_simple [::AI_local n f [::AI_trap]] [::AI_trap]
-  | rs_return :
-      forall n (i: labelidx) vs es (lh: lholed i) f,
-        const_list vs ->
-        length vs = n ->
-        lfilled lh (vs ++ [::AI_basic BI_return]) es ->
-        reduce_simple [::AI_local n f es] vs
-  | rs_tee_local :
-      forall i v,
-        is_const v ->
-        reduce_simple [::v; AI_basic (BI_local_tee i)] [::v; v; AI_basic (BI_local_set i)]
-  | rs_trap :
-      forall es (lh: lholed 0),
-        es <> [::AI_trap] ->
-        lfilled lh [::AI_trap] es ->
-        reduce_simple es [::AI_trap]
-  .
-
+| rs_label_const :
+  forall n es vs,
+    const_list vs ->
+    reduce_simple [::AI_label n es vs] vs
+| rs_label_trap :
+  forall n es,
+    reduce_simple [::AI_label n es [::AI_trap]] [::AI_trap]
+| rs_br :
+  forall n vs es (i: labelidx) LI (lh: lholed (N.to_nat i)),
+    const_list vs ->
+    length vs = n ->
+    lfilled lh (vs ++ [::AI_basic (BI_br i)]) LI ->
+    reduce_simple [::AI_label n es LI] (vs ++ es)
+| rs_br_if_false :
+  forall n i,
+    n = Wasm_int.int_zero i32m ->
+    reduce_simple [::$VA (VAL_int32 n); AI_basic (BI_br_if i)] [::]
+| rs_br_if_true :
+  forall n i,
+    n <> Wasm_int.int_zero i32m ->
+    reduce_simple [::$VA (VAL_int32 n); AI_basic (BI_br_if i)] [::AI_basic (BI_br i)]
+| rs_br_table :
+  forall iss c i j,
+    length iss > Wasm_int.nat_of_uint i32m c ->
+    List.nth_error iss (Wasm_int.nat_of_uint i32m c) = Some j ->
+    reduce_simple [::$VA (VAL_int32 c); AI_basic (BI_br_table iss i)] [::AI_basic (BI_br j)]
+| rs_br_table_length :
+  forall iss c i,
+    length iss <= (Wasm_int.nat_of_uint i32m c) ->
+    reduce_simple [::$VA (VAL_int32 c); AI_basic (BI_br_table iss i)] [::AI_basic (BI_br i)]
+| rs_local_const :
+  forall es n f,
+    const_list es ->
+    length es = n ->
+    reduce_simple [::AI_local n f es] es
+| rs_local_trap :
+  forall n f,
+    reduce_simple [::AI_local n f [::AI_trap]] [::AI_trap]
+| rs_return :
+  forall n (i: labelidx) vs es (lh: lholed (N.to_nat i)) f,
+    const_list vs ->
+    length vs = n ->
+    lfilled lh (vs ++ [::AI_basic BI_return]) es ->
+    reduce_simple [::AI_local n f es] vs
+| rs_tee_local :
+  forall i v,
+    is_const v ->
+    reduce_simple [::v; AI_basic (BI_local_tee i)] [::v; v; AI_basic (BI_local_set i)]
+| rs_trap :
+  forall es (lh: lholed 0),
+    es <> [::AI_trap] ->
+    lfilled lh [::AI_trap] es ->
+    reduce_simple es [::AI_trap]
+.
 
 Inductive reduce : host_state -> store_record -> frame -> list administrative_instruction ->
                    host_state -> store_record -> frame -> list administrative_instruction -> Prop :=
-  | r_simple :
-      forall e e' s f hs,
-        reduce_simple e e' ->
-        reduce hs s f e hs s f e'
-  | r_block :
-    forall hs s f vs es n m tb t1s t2s,
-      expand f.(f_inst) tb = Some (Tf t1s t2s) ->
-      const_list vs ->
-      length vs = n ->
-      length t1s = n ->
-      length t2s = m ->
-      reduce hs s f (vs ++ [::AI_basic (BI_block tb es)]) hs s f [::AI_label m [::] (vs ++ to_e_list es)]
-  | rs_loop :
-      forall hs s f vs es n m tb t1s t2s,
-      expand f.(f_inst) tb = Some (Tf t1s t2s) ->
-      const_list vs ->
-      length vs = n ->
-      length t1s = n ->
-      length t2s = m ->
-      reduce hs s f (vs ++ [::AI_basic (BI_loop tb es)]) hs s f [::AI_label n [::AI_basic (BI_loop tb es)] (vs ++ to_e_list es)]
-  | rs_if_false :
-    forall hs s f c vs es1 es2 n m tb t1s t2s,
-      expand f.(f_inst) tb = Some (Tf t1s t2s) ->
-      c = Wasm_int.int_zero i32m ->
-      const_list vs ->
-      length vs = m ->
-      length t1s = m ->
-      length t2s = n ->
-      reduce hs s f (vs ++ [::$VA (VAL_int32 c); AI_basic (BI_if tb es1 es2)]) hs s f [::AI_label n [::] (vs ++ to_e_list es2)]
-  | rs_if_true :
-    forall hs s f c vs es1 es2 n m tb t1s t2s,
-      expand f.(f_inst) tb = Some (Tf t1s t2s) ->
-      c <> Wasm_int.int_zero i32m ->
-      const_list vs ->
-      length vs = m ->
-      length t1s = m ->
-      length t2s = n ->
-      reduce hs s f (vs ++ [::$VA (VAL_int32 c); AI_basic (BI_if tb es1 es2)]) hs s f [::AI_label n [::] (vs ++ to_e_list es1)]
-  (** calling operations **)
-  | r_call :
-      forall s f (i: funcidx) a hs,
-        List.nth_error f.(f_inst).(inst_funcs) i = Some a ->
-        reduce hs s f [::AI_basic (BI_call i)] hs s f [::AI_invoke a]
-  | r_call_indirect_success :
-      forall s f x (y: typeidx) a cl i hs,
-        stab_elem s f.(f_inst) x (Wasm_int.nat_of_uint i32m i) = Some (VAL_ref_func a) ->
-        List.nth_error s.(s_funcs) a = Some cl ->
-        List.nth_error f.(f_inst).(inst_types) y = Some (cl_type cl) ->
-        reduce hs s f [::$VA (VAL_int32 i); AI_basic (BI_call_indirect x y)] hs s f [::AI_invoke a]
-  | r_call_indirect_failure1 :
-      forall s f x (y: typeidx) a cl i hs,
-        stab_elem s f.(f_inst) x (Wasm_int.nat_of_uint i32m i) = Some (VAL_ref_func a) ->
-        List.nth_error s.(s_funcs) a = Some cl ->
-        List.nth_error f.(f_inst).(inst_types) y <> Some (cl_type cl) ->
-        reduce hs s f [::$VA (VAL_int32 i); AI_basic (BI_call_indirect x y)] hs s f [::AI_trap]
-  | r_call_indirect_failure2 :
-      forall s f x (y: typeidx) a i hs,
-        stab_elem s f.(f_inst) x (Wasm_int.nat_of_uint i32m i) = Some (VAL_ref_func a) ->
-        List.nth_error s.(s_funcs) a = None ->
-        reduce hs s f [::$VA (VAL_int32 i); AI_basic (BI_call_indirect x y)] hs s f [::AI_trap]
-  | r_call_indirect_failure3 :
-      forall s f x (y: typeidx) i hs,
-        stab_elem s f.(f_inst) x (Wasm_int.nat_of_uint i32m i) = None ->
-        reduce hs s f [::$VA (VAL_int32 i); AI_basic (BI_call_indirect x y)] hs s f [::AI_trap]
-  | r_call_indirect_failure4 :
-      forall s f x (y: typeidx) i hs t,
-        stab_elem s f.(f_inst) x (Wasm_int.nat_of_uint i32m i) = Some (VAL_ref_null t) ->
-        reduce hs s f [::$VA (VAL_int32 i); AI_basic (BI_call_indirect x y)] hs s f [::AI_trap]
-  | r_invoke_native :
-      forall a cl t1s t2s ts es ves vcs n m k zs s f f' i hs,
-        List.nth_error s.(s_funcs) (N.to_nat a) = Some cl ->
-        cl = FC_func_native i (Tf t1s t2s) ts es ->
-        ves = v_to_e_list vcs ->
-        length vcs = n ->
-        length ts = k ->
-        length t1s = n ->
-        length t2s = m ->
-        n_zeros ts = zs ->
-        f'.(f_inst) = i ->
-        f'.(f_locs) = vcs ++ zs ->
-        reduce hs s f (ves ++ [::AI_invoke a]) hs s f [::AI_local m f' [::AI_label m [::] (to_e_list es)]]
-  | r_invoke_host_success :
-      forall a cl h t1s t2s ves vcs m n s s' r f hs hs',
-        List.nth_error s.(s_funcs) (N.to_nat a) = Some cl ->
-        cl = FC_func_host (Tf t1s t2s) h ->
-        ves = v_to_e_list vcs ->
-        length vcs = n ->
-        length t1s = n ->
-        length t2s = m ->
-        host_application hs s (Tf t1s t2s) h vcs hs' (Some (s', r)) ->
-        reduce hs s f (ves ++ [::AI_invoke a]) hs' s' f (result_to_stack r)
-  | r_invoke_host_diverge :
-      forall a cl t1s t2s h ves vcs n m s f hs hs',
-        List.nth_error s.(s_funcs) (N.to_nat a) = Some cl ->
-        cl = FC_func_host (Tf t1s t2s) h ->
-        ves = v_to_e_list vcs ->
-        length vcs = n ->
-        length t1s = n ->
-        length t2s = m ->
-        host_application hs s (Tf t1s t2s) h vcs hs' None ->
-        reduce hs s f (ves ++ [::AI_invoke a]) hs' s f (ves ++ [::AI_invoke a])
+| r_simple :
+  forall e e' s f hs,
+    reduce_simple e e' ->
+    reduce hs s f e hs s f e'
+| r_block :
+  forall hs s f vs es n m tb t1s t2s,
+    expand f.(f_inst) tb = Some (Tf t1s t2s) ->
+    const_list vs ->
+    length vs = n ->
+    length t1s = n ->
+    length t2s = m ->
+    reduce hs s f (vs ++ [::AI_basic (BI_block tb es)]) hs s f [::AI_label m [::] (vs ++ to_e_list es)]
+| rs_loop :
+  forall hs s f vs es n m tb t1s t2s,
+    expand f.(f_inst) tb = Some (Tf t1s t2s) ->
+    const_list vs ->
+    length vs = n ->
+    length t1s = n ->
+    length t2s = m ->
+    reduce hs s f (vs ++ [::AI_basic (BI_loop tb es)]) hs s f [::AI_label n [::AI_basic (BI_loop tb es)] (vs ++ to_e_list es)]
+| rs_if_false :
+  forall hs s f c vs es1 es2 n m tb t1s t2s,
+    expand f.(f_inst) tb = Some (Tf t1s t2s) ->
+    c = Wasm_int.int_zero i32m ->
+    const_list vs ->
+    length vs = m ->
+    length t1s = m ->
+    length t2s = n ->
+    reduce hs s f (vs ++ [::$VA (VAL_int32 c); AI_basic (BI_if tb es1 es2)]) hs s f [::AI_label n [::] (vs ++ to_e_list es2)]
+| rs_if_true :
+  forall hs s f c vs es1 es2 n m tb t1s t2s,
+    expand f.(f_inst) tb = Some (Tf t1s t2s) ->
+    c <> Wasm_int.int_zero i32m ->
+    const_list vs ->
+    length vs = m ->
+    length t1s = m ->
+    length t2s = n ->
+    reduce hs s f (vs ++ [::$VA (VAL_int32 c); AI_basic (BI_if tb es1 es2)]) hs s f [::AI_label n [::] (vs ++ to_e_list es1)]
+(** calling operations **)
+| r_call :
+  forall s f (i: funcidx) a hs,
+    List.nth_error f.(f_inst).(inst_funcs) (N.to_nat i) = Some a ->
+    reduce hs s f [::AI_basic (BI_call i)] hs s f [::AI_invoke a]
+| r_call_indirect_success :
+  forall s f x (y: typeidx) a cl i hs,
+    stab_elem s f.(f_inst) x (Wasm_int.nat_of_uint i32m i) = Some (VAL_ref_func a) ->
+    List.nth_error s.(s_funcs) (N.to_nat a) = Some cl ->
+    List.nth_error f.(f_inst).(inst_types) (N.to_nat y) = Some (cl_type cl) ->
+    reduce hs s f [::$VA (VAL_int32 i); AI_basic (BI_call_indirect x y)] hs s f [::AI_invoke a]
+| r_call_indirect_failure1 :
+  forall s f x (y: typeidx) a cl i hs,
+    stab_elem s f.(f_inst) x (Wasm_int.nat_of_uint i32m i) = Some (VAL_ref_func a) ->
+    List.nth_error s.(s_funcs) (N.to_nat a) = Some cl ->
+    List.nth_error f.(f_inst).(inst_types) (N.to_nat y) <> Some (cl_type cl) ->
+    reduce hs s f [::$VA (VAL_int32 i); AI_basic (BI_call_indirect x y)] hs s f [::AI_trap]
+| r_call_indirect_failure2 :
+  forall s f x (y: typeidx) a i hs,
+    stab_elem s f.(f_inst) x (Wasm_int.nat_of_uint i32m i) = Some (VAL_ref_func a) ->
+    List.nth_error s.(s_funcs) (N.to_nat a) = None ->
+    reduce hs s f [::$VA (VAL_int32 i); AI_basic (BI_call_indirect x y)] hs s f [::AI_trap]
+| r_call_indirect_failure3 :
+  forall s f x (y: typeidx) i hs,
+    stab_elem s f.(f_inst) x (Wasm_int.nat_of_uint i32m i) = None ->
+    reduce hs s f [::$VA (VAL_int32 i); AI_basic (BI_call_indirect x y)] hs s f [::AI_trap]
+| r_call_indirect_failure4 :
+  forall s f x (y: typeidx) i hs t,
+    stab_elem s f.(f_inst) x (Wasm_int.nat_of_uint i32m i) = Some (VAL_ref_null t) ->
+    reduce hs s f [::$VA (VAL_int32 i); AI_basic (BI_call_indirect x y)] hs s f [::AI_trap]
+| r_invoke_native :
+  forall a cl t1s t2s ts es ves vcs n m k zs s f f' i hs,
+    List.nth_error s.(s_funcs) (N.to_nat a) = Some cl ->
+    cl = FC_func_native i (Tf t1s t2s) ts es ->
+    ves = v_to_e_list vcs ->
+    length vcs = n ->
+    length ts = k ->
+    length t1s = n ->
+    length t2s = m ->
+    n_zeros ts = zs ->
+    f'.(f_inst) = i ->
+    f'.(f_locs) = vcs ++ zs ->
+    reduce hs s f (ves ++ [::AI_invoke a]) hs s f [::AI_local m f' [::AI_label m [::] (to_e_list es)]]
+| r_invoke_host_success :
+  forall a cl h t1s t2s ves vcs m n s s' r f hs hs',
+    List.nth_error s.(s_funcs) (N.to_nat a) = Some cl ->
+    cl = FC_func_host (Tf t1s t2s) h ->
+    ves = v_to_e_list vcs ->
+    length vcs = n ->
+    length t1s = n ->
+    length t2s = m ->
+    host_application hs s (Tf t1s t2s) h vcs hs' (Some (s', r)) ->
+    reduce hs s f (ves ++ [::AI_invoke a]) hs' s' f (result_to_stack r)
+| r_invoke_host_diverge :
+  forall a cl t1s t2s h ves vcs n m s f hs hs',
+    List.nth_error s.(s_funcs) (N.to_nat a) = Some cl ->
+    cl = FC_func_host (Tf t1s t2s) h ->
+    ves = v_to_e_list vcs ->
+    length vcs = n ->
+    length t1s = n ->
+    length t2s = m ->
+    host_application hs s (Tf t1s t2s) h vcs hs' None ->
+    reduce hs s f (ves ++ [::AI_invoke a]) hs' s f (ves ++ [::AI_invoke a])
 
-  (** get, set, load, and store operations **)
-  | r_local_get :
-      forall f v j s hs,
-        List.nth_error f.(f_locs) (N.to_nat j) = Some v ->
-        reduce hs s f [::AI_basic (BI_local_get j)] hs s f [::AI_basic (BI_const v)]
-  | r_local_set :
-      forall f f' i v s vd hs,
-        f'.(f_inst) = f.(f_inst) ->
-        N.to_nat i < length f.(f_locs) ->
-        f'.(f_locs) = set_nth vd f.(f_locs) (N.to_nat i) v ->
-        reduce hs s f [::AI_basic (BI_const v); AI_basic (BI_local_set i)] hs s f' [::]
-  | r_global_get :
-      forall s f i v hs,
-        sglob_val s f.(f_inst) (N.to_nat i) = Some v ->
-        reduce hs s f [::AI_basic (BI_global_get i)] hs s f [::AI_basic (BI_const v)]
-  | r_global_set :
-      forall s f i v s' hs,
-        supdate_glob s f.(f_inst) (N.to_nat i) v = Some s' ->
-        reduce hs s f [::AI_basic (BI_const v); AI_basic (BI_global_set i)] hs s' f [::]
-               
-  (** table **)
-  | r_table_get_success :
-    forall x i tabv s f hs,
-      stab_elem s f.(f_inst) x (Wasm_int.nat_of_uint i32m i) = Some tabv ->
-      reduce hs s f [::$VA (VAL_int32 i); AI_basic (BI_table_get x)] hs s f [::AI_basic (BI_const (VAL_ref tabv))]
-  | r_table_get_failure :
-    forall x i s f hs,
-      stab_elem s f.(f_inst) x (Wasm_int.nat_of_uint i32m i) = None ->
-      reduce hs s f [::$VA (VAL_int32 i); AI_basic (BI_table_get x)] hs s f [::AI_trap]
-  | r_table_set_success :
-    forall x i tabv s s' f hs,
-      stab_update s f.(f_inst) x (Wasm_int.nat_of_uint i32m i) tabv = Some s' ->
-      reduce hs s f [::$VA (VAL_int32 i); AI_basic (BI_const (VAL_ref tabv)); AI_basic (BI_table_set x)] hs s' f [::]
-  | r_table_set_failure :
-    forall x i tabv s s' f hs,
-      stab_update s f.(f_inst) x (Wasm_int.nat_of_uint i32m i) tabv = None ->
-      reduce hs s f [::$VA (VAL_int32 i); AI_basic (BI_const (VAL_ref tabv)); AI_basic (BI_table_set x)] hs s' f [::]
-             
-  (** memory **)
-  | r_load_success :
-    forall s i f t bs k a off m hs,
-      smem_ind s f.(f_inst) = Some i ->
-      List.nth_error s.(s_mems) i = Some m ->
-      load m (Wasm_int.N_of_uint i32m k) off (tnum_length t) = Some bs ->
-      reduce hs s f [::$VA (VAL_int32 k); AI_basic (BI_load t None a off)] hs s f [::$VA (wasm_deserialise bs t)]
-  | r_load_failure :
-    forall s i f t k a off m hs,
-      smem_ind s f.(f_inst) = Some i ->
-      List.nth_error s.(s_mems) i = Some m ->
-      load m (Wasm_int.N_of_uint i32m k) off (tnum_length t) = None ->
-      reduce hs s f [::$VA (VAL_int32 k); AI_basic (BI_load t None a off)] hs s f [::AI_trap]
-  | r_load_packed_success :
-    forall s i f t tp k a off m bs sx hs,
-      smem_ind s f.(f_inst) = Some i ->
-      List.nth_error s.(s_mems) i = Some m ->
-      load_packed sx m (Wasm_int.N_of_uint i32m k) off (tp_length tp) (tnum_length t) = Some bs ->
-      reduce hs s f [::$VA (VAL_int32 k); AI_basic (BI_load t (Some (tp, sx)) a off)] hs s f [::$VA (wasm_deserialise bs t)]
-  | r_load_packed_failure :
-    forall s i f t tp k a off m sx hs,
-      smem_ind s f.(f_inst) = Some i ->
-      List.nth_error s.(s_mems) i = Some m ->
-      load_packed sx m (Wasm_int.N_of_uint i32m k) off (tp_length tp) (tnum_length t) = None ->
-      reduce hs s f [::$VA (VAL_int32 k); AI_basic (BI_load t (Some (tp, sx)) a off)] hs s f [::AI_trap]
-  | r_store_success :
-    forall t v s i f mem' k a off m hs,
-      typeof_num v = t ->
-      smem_ind s f.(f_inst) = Some i ->
-      List.nth_error s.(s_mems) i = Some m ->
-      store m (Wasm_int.N_of_uint i32m k) off (bits v) (tnum_length t) = Some mem' ->
-      reduce hs s f [::$VA (VAL_int32 k); $VA v; AI_basic (BI_store t None a off)] hs (upd_s_mem s (set_nth mem' s.(s_mems) i mem')) f [::]
-  | r_store_failure :
-    forall t v s i f m k off a hs,
-      typeof_num v = t ->
-      smem_ind s f.(f_inst) = Some i ->
-      List.nth_error s.(s_mems) i = Some m ->
-      store m (Wasm_int.N_of_uint i32m k) off (bits v) (tnum_length t) = None ->
-      reduce hs s f [::$VA (VAL_int32 k); $VA v; AI_basic (BI_store t None a off)] hs s f [::AI_trap]
-  | r_store_packed_success :
-    forall t v s i f m k off a mem' tp hs,
-      typeof_num v = t ->
-      smem_ind s f.(f_inst) = Some i ->
-      List.nth_error s.(s_mems) i = Some m ->
-      store_packed m (Wasm_int.N_of_uint i32m k) off (bits v) (tp_length tp) = Some mem' ->
-      reduce hs s f [::$VA (VAL_int32 k); $VA v; AI_basic (BI_store t (Some tp) a off)] hs (upd_s_mem s (set_nth mem' s.(s_mems) i mem')) f [::]
-  | r_store_packed_failure :
-    forall t v s i f m k off a tp hs,
-      typeof_num v = t ->
-      smem_ind s f.(f_inst) = Some i ->
-      List.nth_error s.(s_mems) i = Some m ->
-      store_packed m (Wasm_int.N_of_uint i32m k) off (bits v) (tp_length tp) = None ->
-      reduce hs s f [::$VA (VAL_int32 k); $VA v; AI_basic (BI_store t (Some tp) a off)] hs s f [::AI_trap]
-  | r_memory_size :
-      forall i f m n s hs,
-        smem_ind s f.(f_inst) = Some i ->
-        List.nth_error s.(s_mems) i = Some m ->
-        mem_size m = n ->
-        reduce hs s f [::AI_basic (BI_memory_size)] hs s f [::$VA (VAL_int32 (Wasm_int.int_of_Z i32m (Z.of_nat n)))]
-  | r_memory_grow_success :
-    forall s i f m n mem' c hs,
-      smem_ind s f.(f_inst) = Some i ->
-      List.nth_error s.(s_mems) i = Some m ->
-      mem_size m = n ->
-      mem_grow m (Wasm_int.N_of_uint i32m c) = Some mem' ->
-      reduce hs s f [::$VA (VAL_int32 c); AI_basic BI_memory_grow] hs (upd_s_mem s (set_nth mem' s.(s_mems) i mem')) f [::$VA (VAL_int32 (Wasm_int.int_of_Z i32m (Z.of_nat n)))]
-  | r_memory_grow_failure :
-      forall i f m n s c hs,
-        smem_ind s f.(f_inst) = Some i ->
-        List.nth_error s.(s_mems) i = Some m ->
-        mem_size m = n ->
-        reduce hs s f [::$VA (VAL_int32 c); AI_basic BI_memory_grow] hs s f [::$VA (VAL_int32 int32_minus_one)]
-  (** label and local **)
-  | r_label :
-      forall k s f es les s' f' es' les' (lh: lholed k) hs hs',
-        reduce hs s f es hs' s' f' es' ->
-        lfilled lh es les ->
-        lfilled lh es' les' ->
-        reduce hs s f les hs' s' f' les'
-  | r_local :
-      forall s f es s' f' es' n f0 hs hs',
-        reduce hs s f es hs' s' f' es' ->
-        reduce hs s f0 [::AI_local n f es] hs' s' f0 [::AI_local n f' es']
-  .
+(** get, set, load, and store operations **)
+| r_local_get :
+  forall f v j s hs,
+    List.nth_error f.(f_locs) (N.to_nat j) = Some v ->
+    reduce hs s f [::AI_basic (BI_local_get j)] hs s f [::AI_basic (BI_const v)]
+| r_local_set :
+  forall f f' i v s vd hs,
+    f'.(f_inst) = f.(f_inst) ->
+    N.to_nat i < length f.(f_locs) ->
+    f'.(f_locs) = set_nth vd f.(f_locs) (N.to_nat i) v ->
+    reduce hs s f [::AI_basic (BI_const v); AI_basic (BI_local_set i)] hs s f' [::]
+| r_global_get :
+  forall s f i v hs,
+    sglob_val s f.(f_inst) (N.to_nat i) = Some v ->
+    reduce hs s f [::AI_basic (BI_global_get i)] hs s f [::AI_basic (BI_const v)]
+| r_global_set :
+  forall s f i v s' hs,
+    supdate_glob s f.(f_inst) (N.to_nat i) v = Some s' ->
+    reduce hs s f [::AI_basic (BI_const v); AI_basic (BI_global_set i)] hs s' f [::]
+           
+(** table **)
+| r_table_get_success :
+  forall x i tabv s f hs,
+    stab_elem s f.(f_inst) x (Wasm_int.nat_of_uint i32m i) = Some tabv ->
+    reduce hs s f [::$VA (VAL_int32 i); AI_basic (BI_table_get x)] hs s f [::AI_basic (BI_const (VAL_ref tabv))]
+| r_table_get_failure :
+  forall x i s f hs,
+    stab_elem s f.(f_inst) x (Wasm_int.nat_of_uint i32m i) = None ->
+    reduce hs s f [::$VA (VAL_int32 i); AI_basic (BI_table_get x)] hs s f [::AI_trap]
+| r_table_set_success :
+  forall x i tabv s s' f hs,
+    stab_update s f.(f_inst) x (Wasm_int.nat_of_uint i32m i) tabv = Some s' ->
+    reduce hs s f [::$VA (VAL_int32 i); AI_basic (BI_const (VAL_ref tabv)); AI_basic (BI_table_set x)] hs s' f [::]
+| r_table_set_failure :
+  forall x i tabv s s' f hs,
+    stab_update s f.(f_inst) x (Wasm_int.nat_of_uint i32m i) tabv = None ->
+    reduce hs s f [::$VA (VAL_int32 i); AI_basic (BI_const (VAL_ref tabv)); AI_basic (BI_table_set x)] hs s' f [::]
+| r_table_size :
+  forall x tab sz s s' f hs,
+    stab s f.(f_inst) x = Some tab ->
+    tab_size tab = sz ->
+    reduce hs s f [:: AI_basic (BI_table_size x)] hs s' f [::$VA (VAL_int32 (Wasm_int.int_of_Z i32m (Z.of_nat sz)))]
+| r_table_grow_success :
+  forall x n tab sz tabinit s s' f hs,
+    stab s f.(f_inst) x = Some tab ->
+    tab_size tab = sz ->
+    stab_grow s f.(f_inst) x (Wasm_int.N_of_uint i32m n) tabinit = Some s' ->
+    reduce hs s f [::AI_basic (BI_const (VAL_ref tabinit)); $VA (VAL_int32 n); AI_basic (BI_table_set x)]
+      hs s' f [::$VA (VAL_int32 (Wasm_int.int_of_Z i32m (Z.of_nat sz)))]
+| r_table_grow_failure :
+  forall x n tab sz tabinit s s' f hs,
+    stab s f.(f_inst) x = Some tab ->
+    tab_size tab = sz ->
+    reduce hs s f [::AI_basic (BI_const (VAL_ref tabinit)); $VA (VAL_int32 n); AI_basic (BI_table_set x)]
+      hs s' f [::$VA (VAL_int32 int32_minus_one)]
+| r_table_fill_bound :
+  forall x i n tab tabv s s' f hs,
+    stab s f.(f_inst) x = Some tab ->
+    (Wasm_int.N_of_uint i32m i) + (Wasm_int.N_of_uint i32m n) > tab_size tab ->
+    reduce hs s f [::$VA (VAL_int32 i); AI_basic (BI_const (VAL_ref tabv)); $VA (VAL_int32 n); AI_basic (BI_table_fill x)]
+      hs s' f [::AI_trap]
+| r_table_fill_return :
+  forall x i n tab tabv s f hs,
+    stab s f.(f_inst) x = Some tab ->
+    (Wasm_int.N_of_uint i32m i) + (Wasm_int.N_of_uint i32m n) <= tab_size tab ->
+    n = Wasm_int.int_zero i32m ->
+    reduce hs s f [::$VA (VAL_int32 i); AI_basic (BI_const (VAL_ref tabv)); $VA (VAL_int32 n); AI_basic (BI_table_fill x)]
+      hs s f [::]
+| r_table_fill_step :
+  forall x i n tab tabv n' i' s f hs,
+    stab s f.(f_inst) x = Some tab ->
+    (Wasm_int.N_of_uint i32m i) + (Wasm_int.N_of_uint i32m n) <= tab_size tab ->
+    n <> Wasm_int.int_zero i32m ->
+    Wasm_int.N_of_uint i32m n' = N.sub (Wasm_int.N_of_uint i32m n) 1 ->
+    Wasm_int.N_of_uint i32m i' = N.add (Wasm_int.N_of_uint i32m i) 1 ->
+    reduce hs s f [::$VA (VAL_int32 i); AI_basic (BI_const (VAL_ref tabv)); $VA (VAL_int32 n); AI_basic (BI_table_fill x)]
+      hs s f [::$VA (VAL_int32 i); AI_basic (BI_const (VAL_ref tabv)); AI_basic (BI_table_set x);
+              $VA (VAL_int32 i'); AI_basic (BI_const (VAL_ref tabv)); $VA (VAL_int32 n'); AI_basic (BI_table_fill x)]
+| r_table_copy_bound :
+  forall x y src dst n tabx taby s f hs,
+    stab s f.(f_inst) x = Some tabx ->
+    stab s f.(f_inst) y = Some taby ->
+    (((Wasm_int.N_of_uint i32m src) + (Wasm_int.N_of_uint i32m n) > tab_size taby) \/
+       ((Wasm_int.N_of_uint i32m dst) + (Wasm_int.N_of_uint i32m n) > tab_size tabx)) ->
+    reduce hs s f [::$VA (VAL_int32 dst); $VA (VAL_int32 src); $VA (VAL_int32 n); AI_basic (BI_table_copy x y)]
+      hs s f [::AI_trap]
+| r_table_copy_return :
+  forall x y src dst n tabx taby s f hs,
+    stab s f.(f_inst) x = Some tabx ->
+    stab s f.(f_inst) y = Some taby ->
+    ((Wasm_int.N_of_uint i32m src) + (Wasm_int.N_of_uint i32m n) <= tab_size taby) ->
+    ((Wasm_int.N_of_uint i32m dst) + (Wasm_int.N_of_uint i32m n) <= tab_size tabx) ->
+    n = Wasm_int.int_zero i32m ->
+    reduce hs s f [::$VA (VAL_int32 dst); $VA (VAL_int32 src); $VA (VAL_int32 n); AI_basic (BI_table_copy x y)]
+      hs s f [::]
+| r_table_copy_forward :
+  forall x y src dst n tabx taby src' dst' n' s f hs,
+    stab s f.(f_inst) x = Some tabx ->
+    stab s f.(f_inst) y = Some taby ->
+    ((Wasm_int.N_of_uint i32m src) + (Wasm_int.N_of_uint i32m n) <= tab_size taby) ->
+    ((Wasm_int.N_of_uint i32m dst) + (Wasm_int.N_of_uint i32m n) <= tab_size tabx) ->
+    n <> Wasm_int.int_zero i32m ->
+    Wasm_int.N_of_uint i32m dst <= Wasm_int.N_of_uint i32m src ->
+    Wasm_int.N_of_uint i32m n' = N.sub (Wasm_int.N_of_uint i32m n) 1 ->
+    Wasm_int.N_of_uint i32m src' = N.add (Wasm_int.N_of_uint i32m src) 1 ->
+    Wasm_int.N_of_uint i32m dst' = N.add (Wasm_int.N_of_uint i32m dst) 1 ->
+    reduce hs s f [::$VA (VAL_int32 dst); $VA (VAL_int32 src); $VA (VAL_int32 n); AI_basic (BI_table_copy x y)]
+      hs s f [:: $VA (VAL_int32 dst); $VA (VAL_int32 src); AI_basic (BI_table_get y); AI_basic (BI_table_get x);
+              $VA (VAL_int32 dst'); $VA (VAL_int32 src'); $VA (VAL_int32 n'); AI_basic (BI_table_copy x y)]
+| r_table_copy_backward :
+  forall x y src dst n tabx taby src' dst' n' s f hs,
+    stab s f.(f_inst) x = Some tabx ->
+    stab s f.(f_inst) y = Some taby ->
+    ((Wasm_int.N_of_uint i32m src) + (Wasm_int.N_of_uint i32m n) <= tab_size taby) ->
+    ((Wasm_int.N_of_uint i32m dst) + (Wasm_int.N_of_uint i32m n) <= tab_size tabx) ->
+    n <> Wasm_int.int_zero i32m ->
+    Wasm_int.N_of_uint i32m dst > Wasm_int.N_of_uint i32m src ->
+    Wasm_int.N_of_uint i32m n' = N.add (Wasm_int.N_of_uint i32m n) 1 ->
+    Wasm_int.N_of_uint i32m src' = N.sub (Wasm_int.N_of_uint i32m src + Wasm_int.N_of_uint i32m n) 1 ->
+    Wasm_int.N_of_uint i32m dst' = N.sub (Wasm_int.N_of_uint i32m dst + Wasm_int.N_of_uint i32m n) 1 ->
+    reduce hs s f [::$VA (VAL_int32 dst); $VA (VAL_int32 src); $VA (VAL_int32 n); AI_basic (BI_table_copy x y)]
+      hs s f [:: $VA (VAL_int32 dst'); $VA (VAL_int32 src'); AI_basic (BI_table_get y); AI_basic (BI_table_get x);
+              $VA (VAL_int32 dst); $VA (VAL_int32 src); $VA (VAL_int32 n'); AI_basic (BI_table_copy x y)]
+| r_table_init_bound :
+  forall x y src dst n tab elem s f hs,
+    stab s f.(f_inst) x = Some tab ->
+    selem s f.(f_inst) y = Some elem ->
+    (((Wasm_int.N_of_uint i32m src) + (Wasm_int.N_of_uint i32m n) > elem_size elem) \/
+       ((Wasm_int.N_of_uint i32m dst) + (Wasm_int.N_of_uint i32m n) > tab_size tab)) ->
+    reduce hs s f [::$VA (VAL_int32 dst); $VA (VAL_int32 src); $VA (VAL_int32 n); AI_basic (BI_table_init x y)]
+      hs s f [::AI_trap]
+| r_table_init_return :
+  forall x y src dst n tab elem s f hs,
+    stab s f.(f_inst) x = Some tab ->
+    selem s f.(f_inst) y = Some elem ->
+    ((Wasm_int.N_of_uint i32m src) + (Wasm_int.N_of_uint i32m n) <= elem_size elem) ->
+    ((Wasm_int.N_of_uint i32m dst) + (Wasm_int.N_of_uint i32m n) <= tab_size tab) ->
+    n = Wasm_int.int_zero i32m ->
+    reduce hs s f [::$VA (VAL_int32 dst); $VA (VAL_int32 src); $VA (VAL_int32 n); AI_basic (BI_table_init x y)]
+      hs s f [::]
+| r_table_init_step :
+  forall x y src dst n tab elem src' dst' n' v s f hs,
+    stab s f.(f_inst) x = Some tab ->
+    selem s f.(f_inst) y = Some elem ->
+    ((Wasm_int.N_of_uint i32m src) + (Wasm_int.N_of_uint i32m n) <= elem_size elem) ->
+    ((Wasm_int.N_of_uint i32m dst) + (Wasm_int.N_of_uint i32m n) <= tab_size tab) ->
+    n <> Wasm_int.int_zero i32m ->
+    List.nth_error elem.(eleminst_elem) (Wasm_int.N_of_uint i32m src) = Some v ->
+    Wasm_int.N_of_uint i32m n' = N.sub (Wasm_int.N_of_uint i32m n) 1 ->
+    Wasm_int.N_of_uint i32m src' = N.add (Wasm_int.N_of_uint i32m src) 1 ->
+    Wasm_int.N_of_uint i32m dst' = N.add (Wasm_int.N_of_uint i32m dst) 1 ->
+    reduce hs s f [::$VA (VAL_int32 dst); $VA (VAL_int32 src); $VA (VAL_int32 n); AI_basic (BI_table_init x y)]
+      hs s f [:: $VA (VAL_int32 dst); AI_basic (BI_const (VAL_ref v)); AI_basic (BI_table_set x);
+              $VA (VAL_int32 dst'); $VA (VAL_int32 src'); $VA (VAL_int32 n'); AI_basic (BI_table_init x y)]
+| r_elem_drop:
+  forall x hs s f s',
+    selem_drop s f.(f_inst) x = Some s' ->
+    reduce hs s f [::AI_basic (BI_elem_drop x)] hs s' f [::]
+           
+(** memory **)
+| r_load_success :
+  forall s i f t bs k a off m hs,
+    smem_ind s f.(f_inst) = Some i ->
+    List.nth_error s.(s_mems) i = Some m ->
+    load m (Wasm_int.N_of_uint i32m k) off (tnum_length t) = Some bs ->
+    reduce hs s f [::$VA (VAL_int32 k); AI_basic (BI_load t None a off)] hs s f [::$VA (wasm_deserialise bs t)]
+| r_load_failure :
+  forall s i f t k a off m hs,
+    smem_ind s f.(f_inst) = Some i ->
+    List.nth_error s.(s_mems) i = Some m ->
+    load m (Wasm_int.N_of_uint i32m k) off (tnum_length t) = None ->
+    reduce hs s f [::$VA (VAL_int32 k); AI_basic (BI_load t None a off)] hs s f [::AI_trap]
+| r_load_packed_success :
+  forall s i f t tp k a off m bs sx hs,
+    smem_ind s f.(f_inst) = Some i ->
+    List.nth_error s.(s_mems) i = Some m ->
+    load_packed sx m (Wasm_int.N_of_uint i32m k) off (tp_length tp) (tnum_length t) = Some bs ->
+    reduce hs s f [::$VA (VAL_int32 k); AI_basic (BI_load t (Some (tp, sx)) a off)] hs s f [::$VA (wasm_deserialise bs t)]
+| r_load_packed_failure :
+  forall s i f t tp k a off m sx hs,
+    smem_ind s f.(f_inst) = Some i ->
+    List.nth_error s.(s_mems) i = Some m ->
+    load_packed sx m (Wasm_int.N_of_uint i32m k) off (tp_length tp) (tnum_length t) = None ->
+    reduce hs s f [::$VA (VAL_int32 k); AI_basic (BI_load t (Some (tp, sx)) a off)] hs s f [::AI_trap]
+| r_store_success :
+  forall t v s i f mem' k a off m hs,
+    typeof_num v = t ->
+    smem_ind s f.(f_inst) = Some i ->
+    List.nth_error s.(s_mems) i = Some m ->
+    store m (Wasm_int.N_of_uint i32m k) off (bits v) (tnum_length t) = Some mem' ->
+    reduce hs s f [::$VA (VAL_int32 k); $VA v; AI_basic (BI_store t None a off)] hs (upd_s_mem s (set_nth mem' s.(s_mems) i mem')) f [::]
+| r_store_failure :
+  forall t v s i f m k off a hs,
+    typeof_num v = t ->
+    smem_ind s f.(f_inst) = Some i ->
+    List.nth_error s.(s_mems) i = Some m ->
+    store m (Wasm_int.N_of_uint i32m k) off (bits v) (tnum_length t) = None ->
+    reduce hs s f [::$VA (VAL_int32 k); $VA v; AI_basic (BI_store t None a off)] hs s f [::AI_trap]
+| r_store_packed_success :
+  forall t v s i f m k off a mem' tp hs,
+    typeof_num v = t ->
+    smem_ind s f.(f_inst) = Some i ->
+    List.nth_error s.(s_mems) i = Some m ->
+    store_packed m (Wasm_int.N_of_uint i32m k) off (bits v) (tp_length tp) = Some mem' ->
+    reduce hs s f [::$VA (VAL_int32 k); $VA v; AI_basic (BI_store t (Some tp) a off)] hs (upd_s_mem s (set_nth mem' s.(s_mems) i mem')) f [::]
+| r_store_packed_failure :
+  forall t v s i f m k off a tp hs,
+    typeof_num v = t ->
+    smem_ind s f.(f_inst) = Some i ->
+    List.nth_error s.(s_mems) i = Some m ->
+    store_packed m (Wasm_int.N_of_uint i32m k) off (bits v) (tp_length tp) = None ->
+    reduce hs s f [::$VA (VAL_int32 k); $VA v; AI_basic (BI_store t (Some tp) a off)] hs s f [::AI_trap]
+| r_memory_size :
+  forall i f m n s hs,
+    smem_ind s f.(f_inst) = Some i ->
+    List.nth_error s.(s_mems) i = Some m ->
+    mem_size m = n ->
+    reduce hs s f [::AI_basic (BI_memory_size)] hs s f [::$VA (VAL_int32 (Wasm_int.int_of_Z i32m (Z.of_nat n)))]
+| r_memory_grow_success :
+  forall s i f m n mem' c hs,
+    smem_ind s f.(f_inst) = Some i ->
+    List.nth_error s.(s_mems) i = Some m ->
+    mem_size m = n ->
+    mem_grow m (Wasm_int.N_of_uint i32m c) = Some mem' ->
+    reduce hs s f [::$VA (VAL_int32 c); AI_basic BI_memory_grow] hs (upd_s_mem s (set_nth mem' s.(s_mems) i mem')) f [::$VA (VAL_int32 (Wasm_int.int_of_Z i32m (Z.of_nat n)))]
+| r_memory_grow_failure :
+  forall i f m n s c hs,
+    smem_ind s f.(f_inst) = Some i ->
+    List.nth_error s.(s_mems) i = Some m ->
+    mem_size m = n ->
+    reduce hs s f [::$VA (VAL_int32 c); AI_basic BI_memory_grow] hs s f [::$VA (VAL_int32 int32_minus_one)]
+| r_memory_fill_bound:
+  forall s f mem d n v hs,
+    smem s f.(f_inst) = Some mem ->
+    (Wasm_int.N_of_uint i32m d) + (Wasm_int.N_of_uint i32m n) > mem_size mem ->
+    reduce hs s f [::$VA (VAL_int32 d); AI_basic (BI_const v); $VA (VAL_int32 n); AI_basic (BI_memory_fill)]
+           hs s f [::AI_trap]
+| r_memory_fill_return:
+  forall s f mem d n v hs,
+    smem s f.(f_inst) = Some mem ->
+    (Wasm_int.N_of_uint i32m d) + (Wasm_int.N_of_uint i32m n) <= mem_size mem ->
+    n = Wasm_int.int_zero i32m ->
+    reduce hs s f [::$VA (VAL_int32 d); AI_basic (BI_const v); $VA (VAL_int32 n); AI_basic (BI_memory_fill)]
+           hs s f [::]
+| r_memory_fill_step:
+  forall s f mem d n d' n' v hs,
+    smem s f.(f_inst) = Some mem ->
+    (Wasm_int.N_of_uint i32m d) + (Wasm_int.N_of_uint i32m n) <= mem_size mem ->
+    n <> Wasm_int.int_zero i32m ->
+    Wasm_int.N_of_uint i32m n' = N.sub (Wasm_int.N_of_uint i32m n) 1 ->
+    Wasm_int.N_of_uint i32m d' = N.add (Wasm_int.N_of_uint i32m d) 1 ->
+    reduce hs s f [::$VA (VAL_int32 d); AI_basic (BI_const v); $VA (VAL_int32 n); AI_basic (BI_memory_fill)]
+      hs s f [::$VA (VAL_int32 d); AI_basic (BI_const v); AI_basic (BI_store T_i32 (Some Tp_i8) N0 N0);
+                $VA (VAL_int32 d'); AI_basic (BI_const v); $VA (VAL_int32 n'); AI_basic (BI_memory_fill)]
+
+           
+(** label and local **)
+| r_label :
+  forall k s f es les s' f' es' les' (lh: lholed k) hs hs',
+    reduce hs s f es hs' s' f' es' ->
+    lfilled lh es les ->
+    lfilled lh es' les' ->
+    reduce hs s f les hs' s' f' les'
+| r_local :
+  forall s f es s' f' es' n f0 hs hs',
+    reduce hs s f es hs' s' f' es' ->
+    reduce hs s f0 [::AI_local n f es] hs' s' f0 [::AI_local n f' es']
+.
 
 Definition reduce_tuple hs_s_f_es hs'_s'_f'_es' : Prop :=
   let '(hs, s, f, es) := hs_s_f_es in
