theories/properties.v
@@ -16,16 +16,6 @@ Section Host.
 
 Variable host_function : eqType.
 
-(*Let administrative_instruction := administrative_instruction host_function.
-Let const_list : seq administrative_instruction -> bool := @const_list _.
-Let v_to_e_list : seq value -> seq administrative_instruction := @v_to_e_list _.
-Let lfilled := @lfilled host_function.
-Let lfilledInd := @lfilledInd host_function.
-Let es_is_basic := @es_is_basic host_function.
-Let to_e_list := @to_e_list host_function.
-Let e_is_trap := @e_is_trap host_function.
-Let es_is_trap := @es_is_trap host_function.*)
-
 
 Lemma const_list_concat: forall vs1 vs2,
     const_list vs1 ->
@@ -122,15 +112,10 @@ Qed.
 
 Lemma es_is_trapP : forall l, reflect (l = [::AI_trap]) (es_is_trap l).
 Proof.
-  case; first by apply: ReflectF.
-  move=> // a l. case l => //=.
-  - apply: (iffP (e_is_trapP _)); first by elim.
-    by inversion 1.
-  - move=> >. by apply: ReflectF.
+  intros; unfold es_is_trap; by apply (iffP eqP).
 Qed.
 
 
-(* Check with Martin for split_n: it's just take+drop *)
 Lemma split_n_is_take_drop: forall es n,
     split_n es n = (take n es, drop n es).
 Proof.
@@ -140,26 +125,12 @@ Proof.
     + by rewrite IH.
 Qed.
 
-(* Ask Martin *)
-Lemma update_list_at_is_set_nth: forall {X:Type} (l:list X) n x,
-    n < size l ->
-    set_nth x l n x = update_list_at l n x.
-Proof.
-  move => X l n x. move: n. elim: l => //=.
-  move => a l IH n HLen. destruct n => //=.
-  unfold update_list_at. simpl. f_equal. by apply IH.
-Qed.
-
-(* Check with Martin: size is the standard function used in ssreflect.seq; should we
-   change all occurrences of length to size instead? *)
 Lemma length_is_size: forall {X:Type} (l: list X),
     length l = size l.
 Proof.
   move => X l. by elim: l.
 Qed.
 
-(* Very interestingly, the following lemma has EXACTLY the same proof as the
-   lemma split_n_is_take_drop, although they are not related at all! *)
 Lemma v_to_e_take_exchange: forall vs n,
     v_to_e_list (take n vs) = take n (v_to_e_list vs).
 Proof.
@@ -227,70 +198,54 @@ Qed.
 Lemma to_e_list_basic: forall bes,
     es_is_basic (to_e_list bes).
 Proof.
-  induction bes => //=.
-  split => //=.
-  unfold e_is_basic. by eauto.
+  elim => //=; move => be bes IH.
+  apply List.Forall_cons => //.
+  by eexists.
 Qed.
 
 Lemma basic_concat: forall es1 es2,
     es_is_basic (es1 ++ es2) ->
     es_is_basic es1 /\ es_is_basic es2.
 Proof.
-  induction es1 => //=.
-  move => es2 H. destruct H.
-  apply IHes1 in H0. destruct H0.
-  by repeat split => //=.
+  by apply List.Forall_app.
 Qed.
-
+  
 Lemma basic_split: forall es1 es2,
     es_is_basic es1 ->
     es_is_basic es2 ->
     es_is_basic (es1 ++ es2).
 Proof.
-  induction es1 => //=.
-  move => es2 H1 H2.
-  destruct H1.
-  split => //=.
-  by apply IHes1.
+  intros; by apply List.Forall_app.
 Qed.
 
 Lemma const_list_is_basic: forall es,
     const_list es ->
     es_is_basic es.
 Proof.
-  induction es => //=.
-  move => H. move/andP in H. destruct H.
-  split.
-  - destruct a => //.
-    unfold e_is_basic. by eauto.
-  - by apply IHes.                                 
+  induction es; try by intros => //=.
+  move => H. move/andP in H. destruct H as [H Hs].
+  apply IHes in Hs.
+  apply List.Forall_cons => //.
+  destruct a => //.
+  by eexists.
 Qed.
 
 Lemma to_b_list_rev: forall es : seq administrative_instruction,
     rev (to_b_list es) = to_b_list (rev es).
 Proof.
-  induction es => //=.
-  repeat rewrite rev_cons.
-  rewrite IHes.
-  repeat rewrite -cats1.
-  by rewrite to_b_list_concat.
+  unfold to_b_list. intros. by rewrite map_rev.
 Qed.
 
 Lemma vs_to_vts_cat: forall vs1 vs2,
-    vs_to_vts (vs1 ++ vs2) = vs_to_vts vs1 ++ vs_to_vts vs2.
+  vs_to_vts (vs1 ++ vs2) = vs_to_vts vs1 ++ vs_to_vts vs2.
 Proof.
-  induction vs1 => //=.
-  move => vs2. by rewrite IHvs1.
+  by apply map_cat.
 Qed.
   
 Lemma vs_to_vts_rev: forall vs,
-    vs_to_vts (rev vs) = rev (vs_to_vts vs).
+  vs_to_vts (rev vs) = rev (vs_to_vts vs).
 Proof.
-  induction vs => //=.
-  repeat rewrite rev_cons.
-  repeat rewrite -cats1.
-  rewrite vs_to_vts_cat.
-  by rewrite IHvs.
+  unfold vs_to_vts. intros. by rewrite map_rev.
 Qed.
   
 Lemma const_es_exists: forall es,
@@ -300,23 +255,20 @@ Proof.
   induction es => //=.
   - by exists [::].
   - move => HConst.
-    move/andP in HConst. destruct HConst.
+    move/andP in HConst. destruct HConst as [H Hs].
     destruct a => //=. destruct b => //=.
-    edestruct IHes => //=.
-    exists (v :: x). simpl. by rewrite H1.
+    apply IHes in Hs as [vs ->].
+    by exists (v :: vs).
 Qed.
 
 Lemma b_e_elim: forall bes es,
     to_e_list bes = es ->
     bes = to_b_list es /\ es_is_basic es.
 Proof.
-  induction bes; move => es H => //=.
-  - by rewrite -H.
-  - simpl in H. assert (es = to_e_list (a :: bes)) as H1.
-    + by rewrite -H.
-    + rewrite H1. split.
-      -- simpl. f_equal. by apply IHbes.
-      -- by apply to_e_list_basic.
+  move => bes es <-.
+  split; last by apply to_e_list_basic.
+  unfold to_b_list, to_e_list.
+  induction bes => //=; by f_equal.
 Qed.
 
 Lemma e_b_elim: forall bes es,
@@ -324,12 +276,12 @@ Lemma e_b_elim: forall bes es,
     es_is_basic es ->
     es = to_e_list bes.
 Proof.
-  induction bes; move => es H1 H2 => //=.
-  - by destruct es => //=.
-  - destruct es => //=. simpl in H1. simpl in H2. destruct H2.
-    inversion H1; subst.
-    inversion H; subst => //=.
-    f_equal. apply IHbes => //=.
+  move => bes es -> Hbasic.
+  induction es as [ | a es] => //=.
+  unfold es_is_basic in Hbasic.
+  inversion Hbasic as [|?? H Hs]; subst.
+  apply IHes in Hs; rewrite <- Hs.
+  destruct a => //; try by destruct H.
 Qed.
     
 Lemma to_e_list_injective: forall bes bes',
@@ -345,8 +297,7 @@ Qed.
 Lemma to_e_list_cat: forall bes1 bes2,
     to_e_list (bes1 ++ bes2) = to_e_list bes1 ++ to_e_list bes2.
 Proof.
-  induction bes1 => //.
-  move => bes2. simpl. by f_equal.
+  by apply map_cat.
 Qed.
 
 (* Maybe there are better/standard tactics for dealing with these, but I didn't find
@@ -412,7 +363,7 @@ Qed.
 Lemma list_nth_prefix: forall {X:Type} (l1 l2: seq X) x,
     List.nth_error (l1 ++ [::x] ++ l2) (length l1) = Some x.
 Proof.
-  move => X. induction l1 => //=.
+  move => X. by induction l1 => //=.
 Qed.
 
 End Host.
@@ -536,9 +487,8 @@ Ltac basic_inversion :=
          | H: es_is_basic [::] |- _ =>
            clear H
          | H: es_is_basic [::_] |- _ =>
-           let H1 := fresh H in
-           let H2 := fresh H in
-           try by (unfold es_is_basic in H; destruct H as [H1 H2]; inversion H1)
+           let Hcontra := fresh "Hcontra" in
+            try by (inversion H as [|?? Hcontra]; destruct Hcontra as [? Hcontra]; inversion Hcontra)
          | H: e_is_basic _ |- _ =>
            inversion H; try by []
          end.
@@ -566,14 +516,15 @@ Ltac extract_listn :=
   | H: _ :: _ = _ ++ _ |- _ => symmetry in H
          end.
 
+
 Ltac fold_upd_context :=
   lazymatch goal with
   | |- context [upd_local (upd_return ?C ?ret) ?loc] =>
     replace (upd_local (upd_return C ret) loc) with
-        (upd_local_return C ret loc); try by destruct C
+        (upd_local_label_return C loc (tc_label C) ret); try by destruct C
   | |- context [upd_return (upd_local ?C ?ret) ?loc] =>
     replace (upd_return (upd_local C ret) loc) with
-        (upd_local_return C ret loc); try by destruct C
+        (upd_local_label_return C loc (tc_label C) ret); try by destruct C
   end.
 
 
@@ -586,16 +537,10 @@ Variable host_function : eqType.
 
 Let store_record := store_record host_function.
 Let function_closure := function_closure host_function.
-(* Let administrative_instruction := administrative_instruction host_function. 
-Let const_list : seq administrative_instruction -> bool := @const_list _.
-Let v_to_e_list : seq value -> seq administrative_instruction := @v_to_e_list _.
-Let lfilled := @lfilled host_function.
-Let lfilledInd := @lfilledInd host_function.
-Let es_is_basic := @es_is_basic host_function.
-Let to_e_list := @to_e_list host_function.*)
 Let e_typing : store_record -> t_context -> seq administrative_instruction -> function_type -> Prop :=
   @e_typing _.
 
+(*
 Lemma lfilled_collapse1: forall n lh vs es LI l,
     lfilledInd n lh (vs++es) LI ->
     const_list vs ->
@@ -635,19 +580,18 @@ Proof.
     simpl in H0. rewrite cats0 in H0. by apply H0.
   - destruct IHHLF => //. eexists (LH_rec _ _ _ _ _). apply LfilledRec => //. by apply H0.
 Qed.
+ *)
 
-Lemma lfilled_deterministic: forall k lh es les les',
-    lfilledInd k lh es les ->
-    lfilledInd k lh es les' ->
+Lemma lfilled_deterministic: forall k (lh: lholed k) es les les',
+    lfilled lh es les ->
+    lfilled lh es les' ->
     les = les'.
 Proof.
-  move => k lh es les les' HLF HLF'.
-  apply lfilled_Ind_Equivalent in HLF. unfold operations.lfilled in HLF.
-  apply lfilled_Ind_Equivalent in HLF'. unfold operations.lfilled in HLF'.
-  destruct (lfill k lh es) => //.
-  replace les' with l.
-  { move: HLF. by apply/eqseqP. }
-  symmetry. move: HLF'. by apply/eqseqP. 
+  unfold lfilled in *.
+  intros ????? Hlf1 Hlf2.
+  move/eqP in Hlf1.
+  move/eqP in Hlf2.
+  by subst.
 Qed.  
 
 Lemma all_projection: forall {X:Type} f (l:seq X) n x,
@@ -656,7 +600,7 @@ Lemma all_projection: forall {X:Type} f (l:seq X) n x,
     f x.
 Proof.
   move => X f l n x.
-  generalize dependent l.
+  move: l.
   induction n => //; destruct l => //=; move => HF HS; remove_bools_options => //.
   eapply IHn; by eauto.
 Qed.
@@ -668,8 +612,7 @@ Lemma all2_projection: forall {X Y:Type} f (l1:seq X) (l2:seq Y) n x1 x2,
     f x1 x2.
 Proof.
   move => X Y f l1 l2 n.
-  generalize dependent l1.
-  generalize dependent l2.
+  move: l2 l1.
   induction n => //=; move => l2 l1 x1 x2 HALL HN1 HN2.
   - destruct l1 => //=. destruct l2 => //=.
     inversion HN1. inversion HN2. subst. clear HN1. clear HN2.
@@ -709,6 +652,8 @@ Definition lfilled_pickable_rec_gen_measure (LI : seq administrative_instruction
        (fun _ => 0)
        0
        (fun _ => 0)
+       (fun _ => 0)
+       (fun _ => 0)
        (fun _ LI1 LI2 m1 m2 => 1 + TProp.max m2)
        (fun _ _ LI' m => 0)
        LI).
@@ -737,6 +682,7 @@ Proof.
     by apply: leq_maxr.
 Qed.
 
+(*
 Lemma lfilled_pickable_rec_gen_measure_label_r : forall n es LI LI',
   lfilled_pickable_rec_gen_measure LI < lfilled_pickable_rec_gen_measure (AI_label n es LI :: LI').
 Proof.
@@ -873,6 +819,7 @@ Proof.
   - move=> [[vs es''] [E [C _]]]. left. eexists. subst. by constructor.
   - move=> nE. right. move=> [lh I]. apply: nE. inversion I. subst. by repeat eexists.
 Defined.
+ 
 
 (** A helper definition for the decidability of [br_reduce] and [return_reduce]
   (see type_soundness.v). **)
@@ -882,6 +829,7 @@ Definition lfilled_pickable_rec : forall es,
 Proof.
   move=> es D. by apply: lfilled_pickable_rec_gen.
 Defined.
+*)
 
 (* A reformulation of [ety_a] that is easier to be used. *)
 Lemma ety_a': forall s C es ts,
@@ -901,7 +849,7 @@ Lemma bet_weakening_empty_1: forall C es ts t2s,
     be_typing C es (Tf ts (ts ++ t2s)).
 Proof.
   move => C es ts t2s HType.
-  assert (be_typing C es (Tf (ts ++ [::]) (ts ++ t2s))); first by apply bet_weakening.
+  assert (be_typing C es (Tf (ts ++ [::]) (ts ++ t2s))) as H; first by apply bet_weakening.
   by rewrite cats0 in H.
 Qed.
 
@@ -910,7 +858,7 @@ Lemma et_weakening_empty_1: forall s C es ts t2s,
     e_typing s C es (Tf ts (ts ++ t2s)).
 Proof.
   move => s C es ts t2s HType.
-  assert (e_typing s C es (Tf (ts ++ [::]) (ts ++ t2s))); first by apply ety_weakening.
+  assert (e_typing s C es (Tf (ts ++ [::]) (ts ++ t2s))) as H; first by apply ety_weakening.
   by rewrite cats0 in H.
 Qed.
 
@@ -919,7 +867,7 @@ Lemma bet_weakening_empty_2: forall C es ts t1s,
     be_typing C es (Tf (ts ++ t1s) ts).
 Proof.
   move => C es ts t1s HType.
-  assert (be_typing C es (Tf (ts ++ t1s) (ts ++ [::]))); first by apply bet_weakening.
+  assert (be_typing C es (Tf (ts ++ t1s) (ts ++ [::]))) as H; first by apply bet_weakening.
   by rewrite cats0 in H.
 Qed.
 
@@ -928,17 +876,10 @@ Lemma bet_weakening_empty_both: forall C es ts,
     be_typing C es (Tf ts ts).
 Proof.
   move => C es ts HType.
-  assert (be_typing C es (Tf (ts ++ [::]) (ts ++ [::]))); first by apply bet_weakening.
+  assert (be_typing C es (Tf (ts ++ [::]) (ts ++ [::]))) as H; first by apply bet_weakening.
   by rewrite cats0 in H.
 Qed.
 
-(*
-  This is actually very non-trivial to prove, unlike I first thought.
-  The main difficulty arises due to the two rules bet_composition and bet_weakening,
-    which will apply for EVERY hypothesis of be_typing when doing inversion/induction.
-  Moreover, bet_weakening has a reversed inductive structure, so the proof in fact
-    required induction (where one would hardly expect an induction here!).
-*)
 Lemma empty_typing: forall C t1s t2s,
     be_typing C [::] (Tf t1s t2s) ->
     t1s = t2s.
@@ -949,7 +890,6 @@ Proof.
   - f_equal. by eapply IHHType.
 Qed.
 
-(* A convenient lemma to invert e_typing back to be_typing. *)
 Lemma et_to_bet: forall s C es ts,
     es_is_basic es ->
     e_typing s C es ts ->
@@ -991,7 +931,6 @@ Lemma composition_typing_single: forall C es1 e t1s t2s,
 Proof.
   move => C es1 e t1s t2s HType.
   gen_ind_subst HType; extract_listn; auto_prove_bet.
-  + by apply bet_block.
   + by destruct es1 => //=.
   + apply concat_cancel_last in H1. destruct H1. subst.
     by exists [::], t1s0, t2s0, t2s.
@@ -1065,10 +1004,14 @@ Proof.
     repeat split => //=.
     + apply ety_a' => //. apply bet_weakening_empty_both. by apply bet_empty.
     + by apply ety_trap.
-  - (* Local *)
-    exists [::], [::], t2s, [::]. repeat split => //=.
-    + by apply ety_a' => //.
-    + by apply ety_local.
+  - (* External ref *)
+    exists [::], [::], [::T_ref T_externref], [::]. repeat split => //=.
+    + by apply ety_a'.
+    + by apply ety_ref_extern.
+  - (* Funcref *)
+    exists [::], [::], [::T_ref T_funcref], [::]. repeat split => //=.
+    + by apply ety_a'.
+    + by eapply ety_ref; apply H.
   - (* Invoke *)
     exists [::], t1s, t2s, t1s. repeat split => //=.
     + apply ety_a' => //. apply bet_weakening_empty_both. by apply bet_empty.
@@ -1077,6 +1020,10 @@ Proof.
     exists [::], [::], t2s0, [::]. repeat split => //=.
     + by apply ety_a' => //.
     + by eapply ety_label; eauto.
+  - (* Local *)
+    exists [::], [::], t2s, [::]. repeat split => //=.
+    + by apply ety_a' => //.
+    + by apply ety_local.
 Qed.
 
 Lemma e_composition_typing: forall s C es1 es2 t1s t2s,
